\newpage
\chapter{Nonlinear solver}

\noindent Linearization:

\begin{equation} \label{eq:67} 
y = \partial_x f \left(x - x_n \right) + f \left(x_n\right)
\end{equation}

\begin{equation} \label{eq:68} 
0 = S A - M J - C B_r = S A - f
\end{equation}

\begin{align*} 
0 &= \partial_A \left(S A_n - f\right) \left(A_{n+1} - A_n \right) + \left(S A_n - f\right) \\
A_{n+1} &=  A_n  - \partial_A \left(S A_n - f\right)^{-1}  \left(S A_n - f\right)
\end{align*}

\noindent Right hand side $f$ is not dependent on $A$, $\partial_A f = 0$. 

\begin{equation} \label{eq:69} 
A_{n+1} = A_n - \partial_A \left(S A_n \right)^{-1}  \left(S A_n - f\right)
\end{equation}

\noindent Derivative $\partial_A \left(S A \right)$ was already derived in chapter 3, (\ref{eq:64}) and (\ref{eq:65}).


