\newpage
\chapter{Theory}

\section{2D Magnetodynamic equations}

\noindent Cartesian coordinate system $(x,y,z)$

\begin{equation} \label{eq:1}
\nabla \times \left( \frac{1}{\mu} \left( \nabla \times \bm{A} \right) \right) + \gamma \frac{\partial \bm{A}}{\partial t} - \gamma \left( \bm{v} \times \left( \nabla \times \bm{A} \right) \right) = \bm{J}
\end{equation}


\begin{align*} 
\bm{A} &= \left(0,0,A_z\right) \numberthis \label{eq:2} \\
\bm{J} &= \left(0,0,J_z\right) \numberthis \label{eq:3} \\
\bm{v} &= \left(v_x,v_y,0\right) \numberthis \label{eq:4} \\
\bm{B} &= \nabla \times \bm{A} = \left(\partial_y A_x,-\partial_x A_y,0\right) = \left(B_x,B_y,0\right) \numberthis \label{eq:5} \\
\bm{v} \times \bm{B} &= \left(0,0,v_x B_y - v_y B_x\right) \numberthis \label{eq:6}
\end{align*}

\begin{align*}
\bm{A}, \bm{J}, \bm{v}  &= f\left(x,y,t\right) \numberthis \label{eq:7} \\
\mathrm{Linear} \quad \mu, \gamma  &= f\left(x,y\right) \qquad \mathrm{Nonlinear} \quad \mu = f\left(x,y, ||\bm{B}||\right) \numberthis \label{eq:8}
\end{align*}

\section{Boundary condition}

\begin{equation} \label{eq:9} 
A_z\bigg\rvert_{\partial \Omega} = 0
\end{equation}

\section{Initial condition}

\begin{equation} \label{eq:10} 
A_z\bigg\rvert_{t=0} = 0
\end{equation}


\section{Force}

\begin{equation} \label{eq:11} 
T_{ij} = \frac{1}{\mu_0} \left(B_i B_j - \frac{1}{2} B^2 \delta_{ij}\right)
\end{equation}

\begin{equation} \label{eq:12} 
\mathbb{T} = \frac{1}{\mu_0} \begin{pmatrix}
B_x B_x & B_x B_y \\
B_y B_x & B_y B_y \\
\end{pmatrix} - \frac{1}{2\mu_0} \begin{pmatrix}
B_x^2 + B_y^2 & 0 \\
0 & B_x^2 + B_y^2 \\
\end{pmatrix}
\end{equation}

\begin{align*}
\mathrm{3D} \qquad &\bm{F}\left(x,y,z\right) = \oint_{\partial \Omega} \mathbb{T}  \,\mathrm{d}\bm{S} = \int_{\Omega} \left( \nabla \cdot \mathbb{T} \right) \,\mathrm{d}V \numberthis \label{eq:13} \\
\mathrm{2D} \qquad &\bm{F}\left(x,y\right) = L \oint_{\partial \Omega} \mathbb{T}  \,\mathrm{d}\bm{l} = L \int_{\Omega} \left( \nabla \cdot \mathbb{T} \right) \,\mathrm{d}S \numberthis \label{eq:14} \\
\end{align*}

\begin{equation} \label{eq:15} 
\nabla \cdot \mathbb{T} = \frac{1}{\mu_0} \left(\partial_x,\partial_y\right) \begin{pmatrix}
\frac{1}{2} \left(B_x^2 - B_y^2 \right) & B_x B_y \\
B_y B_x & \frac{1}{2} \left(B_y^2 - B_x^2 \right) \\
\end{pmatrix}
\end{equation}

\begin{equation} \label{eq:16} 
\nabla \cdot \mathbb{T} = \frac{1}{\mu_0} \left(\frac{1}{2} \partial_x \left(B_x^2 - B_y^2 \right) + \partial_y \left( B_y B_x \right), \frac{1}{2} \partial_y \left(B_y^2 - B_x^2 \right) + \partial_x \left( B_x B_y \right)\right)
\end{equation}

\begin{align*}
\nabla \cdot \mathbb{T} \left(x\right) = \frac{1}{\mu_0} \left( \partial_x B_x B_x - \partial_x B_y B_y + \partial_y B_y B_x + \partial_y B_x B_y \right) \numberthis \label{eq:17} \\
\nabla \cdot \mathbb{T} \left(y\right) = \frac{1}{\mu_0} \left( \partial_y B_y B_y - \partial_y B_x B_x + \partial_x B_x B_y + \partial_x B_y B_x \right) \numberthis \label{eq:18} \\
\end{align*}